allows comp to java

DynamicArray/src/main/java/DynamicArray_Compile/Vector.java
@@ -1,0 +1,87 @@
+// Class Vector
+// Dafny class Vector compiled into Java
+package DynamicArray_Compile;
+
+import NativeTypes_Compile.*;
+
+@SuppressWarnings({"unchecked", "deprecation"})
+public class Vector<T> {
+  private dafny.TypeDescriptor<T> _td_T;
+  public Vector(dafny.TypeDescriptor<T> _td_T) {
+    this._td_T = _td_T;
+    this.buffer = (Object) _td_T.newArray(0);
+    this.current__capacity = 0;
+    this.current__size = 0;
+  }
+  public java.lang.Object buffer;
+  public int current__capacity;
+  public int current__size;
+  public int get__size()
+  {
+    int x = 0;
+    x = this.current__size;
+    return x;
+  }
+  public T at__index(int index)
+  {
+    @SuppressWarnings({"unchecked", "deprecation"})
+    T x = null;
+    x = _td_T.getArrayElement((this.buffer), (index));
+    return x;
+  }
+  public void extend__buffer(T value)
+  {
+    if (Integer.compareUnsigned(this.current__capacity, Integer.divideUnsigned(NativeTypes_Compile.__default.UINT32__MAX(), 2)) >= 0) {
+      Extern.fatal(dafny.DafnySequence.asString("at max capacity"));
+      return;
+    }
+    java.lang.Object _154_old__buffer;
+    _154_old__buffer = this.buffer;
+    int _155_old__size;
+    _155_old__size = this.current__capacity;
+    (this).current__capacity = (int)  ((_155_old__size) * (2));
+    java.lang.Object _out0;
+    _out0 = Extern.<T>newArrayFill(_td_T, this.current__capacity, value);
+    (this).buffer = _out0;
+    int _156_i;
+    _156_i = 0;
+    goto_0: {
+      while (Integer.compareUnsigned(_156_i, _155_old__size) < 0) {
+        java.lang.Object _arr0 = this.buffer;
+        _td_T.setArrayElement(_arr0, (_156_i),_td_T.getArrayElement((_154_old__buffer), (_156_i)));
+        if ((_156_i) == ((int)  ((_155_old__size) - (1)))) {
+          break goto_0;
+        }
+        _156_i = (int)  ((_156_i) + (1));
+      }
+    }
+  }
+  public void push__back(T value)
+  {
+    if (((int)  ((this.current__size) + (1))) == (this.current__capacity)) {
+      (this).extend__buffer(value);
+    }
+    java.lang.Object _arr1 = this.buffer;
+    int _index0 = this.current__size;
+    _td_T.setArrayElement(_arr1, _index0,value);
+    (this).current__size = (int)  ((this.current__size) + (1));
+  }
+  public void clear()
+  {
+    (this).current__size = 0;
+  }
+  public void __ctor(T default__val)
+  {
+    (this).current__size = 0;
+    (this).current__capacity = Vector.<T>DEFAULT__SIZE(_td_T);
+    java.lang.Object _out1;
+    _out1 = Extern.<T>newArrayFill(_td_T, Vector.<T>DEFAULT__SIZE(_td_T), default__val);
+    (this).buffer = _out1;
+  }
+  public static <T> int DEFAULT__SIZE(dafny.TypeDescriptor<T> _td_T) {
+    return 16;
+  }
+  public static <T> dafny.TypeDescriptor<Vector<T>> _typeDescriptor(dafny.TypeDescriptor<T> _td_T) {
+    return (dafny.TypeDescriptor<Vector<T>>) (dafny.TypeDescriptor<?>) dafny.TypeDescriptor.referenceWithInitializer(Vector.class, () -> (Vector<T>) null);
+  }
+}
