DynamicArray/src/main/java/NativeTypes_Compile/uint32.java
@@ -1,0 +1,19 @@
+// Class uint32
+// Dafny class uint32 compiled into Java
+package NativeTypes_Compile;
+
+
+@SuppressWarnings({"unchecked", "deprecation"})
+public class uint32 {
+  public uint32() {
+  }
+  public static java.util.ArrayList<Integer> IntegerRange(java.math.BigInteger lo, java.math.BigInteger hi) {
+    java.util.ArrayList<Integer> arr = new java.util.ArrayList<>();
+    for (java.math.BigInteger j = lo; j.compareTo(hi) < 0; j = j.add(java.math.BigInteger.ONE)) { arr.add(Integer.valueOf(j.intValue())); }
+    return arr;
+  }
+  private static final dafny.TypeDescriptor<Integer> _TYPE = dafny.TypeDescriptor.intWithDefault(0);
+  public static dafny.TypeDescriptor<Integer> _typeDescriptor() {
+    return (dafny.TypeDescriptor<Integer>) (dafny.TypeDescriptor<?>) _TYPE;
+  }
+}
