DynamicArray/src/test/java/Utils_Compile/DynamicArrayUtils.java
@@ -1,0 +1,16 @@
+// Class DynamicArrayUtils
+// Dafny class DynamicArrayUtils compiled into Java
+package Utils_Compile;
+
+import NativeTypes_Compile.*;
+import DynamicArray_Compile.*;
+
+@SuppressWarnings({"unchecked", "deprecation"})
+public class DynamicArrayUtils {
+  public DynamicArrayUtils() {
+  }
+  private static final dafny.TypeDescriptor<DynamicArrayUtils> _TYPE = dafny.TypeDescriptor.referenceWithInitializer(DynamicArrayUtils.class, () -> (DynamicArrayUtils) null);
+  public static dafny.TypeDescriptor<DynamicArrayUtils> _typeDescriptor() {
+    return (dafny.TypeDescriptor<DynamicArrayUtils>) (dafny.TypeDescriptor<?>) _TYPE;
+  }
+}
