DynamicArray/src/test/java/Utils_Compile/JUnit5.java
@@ -1,0 +1,15 @@
+// Class JUnit5
+// Dafny class JUnit5 compiled into Java
+package Utils_Compile;
+
+import org.junit.jupiter.api.Assertions;
+
+@SuppressWarnings({"unchecked", "deprecation"})
+public class JUnit5 {
+  public JUnit5() {
+  }
+  private static final dafny.TypeDescriptor<JUnit5> _TYPE = dafny.TypeDescriptor.referenceWithInitializer(JUnit5.class, () -> (JUnit5) null);
+  public static dafny.TypeDescriptor<JUnit5> _typeDescriptor() {
+    return (dafny.TypeDescriptor<JUnit5>) (dafny.TypeDescriptor<?>) _TYPE;
+  }
+}
