DynamicArray/dafny-compile-java.sh
@@ -1,0 +1,34 @@
+#!/bin/sh
+
+DOTNET="/usr/bin/dotnet"
+DAFNY="/home/deant4/.vscode-server/extensions/correctnesslab.dafny-vscode-2.0.2/out/resources/dafny/Dafny.dll"
+MODEL="./dafny/DynamicArrayTests.dfy"
+ARGS="/verifyAllModules /compileTarget:java /compile:1 /spillTargetCode:1 /out:DynamicArray"
+
+${DOTNET} ${DAFNY} ${MODEL} $ARGS
+
+rm -rf src/main/java/DynamicArray_Compile
+mv ./DynamicArray-java/DynamicArray_Compile src/main/java/.
+
+rm -rf src/test/java/DynamicArrayTests_Compile
+mv ./DynamicArray-java/DynamicArrayTests_Compile src/test/java/.
+
+##############################################################################
+# Do not move these files as they are "external"                             #
+# and will clobber the test support code.                                    # 
+#                                                                            #
+rm -rf src/test/java/Utils_Compile                                         #
+mv ./DynamicArray-java/Utils_Compile src/test/java/.                           #
+rm -rf src/main/java/NativeTypes_Compile                                         #
+mv ./DynamicArray-java/NativeTypes_Compile src/main/java/.   
+##############################################################################
+
+# TODO: figure out when (if) these are needed
+# rm -rf src/main/java/_System
+# mv ./DynamicArray-java/_System src/main/java/.
+#
+# rm -rf src/main/java/dafny
+# mv ./DynamicArray-java/dafny src/main/java/.
+
+find src/ -name "*.class" | xargs rm -rf
+rm -rf ./DynamicArray-java
